added documentation

papers/protocols/coq/StateMonad.v
@@ -7,18 +7,32 @@
 *)
 
 Require Import FunctionalExtensionality.
+Require Import Arith.
 
-(** First attempt that simply copies the PVS implementation *)
+(** First attempt that simply copies the PVS implementation.  The datatype
+ is not parameterized, but [A] and [S] are specified as a uninterpretted
+ types. *)
 
 Module definition1.
 
 Definition A := nat.
 Definition S := nat.
 
+(** [State] is an algebraic type that encapsulates [state] as done in Haskell
+  and PVS *)
+
 Inductive State :=
   | state : (S -> A * S) -> State.
 
+(** [unit :: A -> M A] has the classical definition of lifting a state into
+  the monad and waiting for an input *)
+
 Definition unit(x:A):State := state(fun (s:S) => (x,s)).
+
+
+(** [bind :: M A -> (A -> M B) -> M B] has the classical definition of taking
+  a monad, running it, and feeding the result into the next monadic expression
+  in sequence. *)
 
 Definition bind(m:State)(f:A -> State):State :=
   (state (fun (s0:S) =>
@@ -40,14 +54,22 @@ Qed.
 End definition1.
 
 (** Second attempt that removes the constructed type in favor of a simple
-    type definition. *)
+    type definition. Coq supports general functions over types.  Thus, we
+    redefine [State] directly as the type [S -> A * S] *)
 
 Module definition2.
 
+(** Still use uninterpretted types for [A] and [S] *)
 Definition A := nat.
 Definition S := nat.
 
+(** [State] is a type that defines the state monad in the classical fashion
+  without using a constructed type *)
+
 Definition State := S -> A * S.
+
+(** Definitions of [unit] and [bind] follow directly from [State].  The
+  [sequence] operation is added in this definition *)
 
 Definition unit(x:A):State := (fun (s:S) => (x,s)).
 
@@ -82,6 +104,8 @@ Proof.
   unfold bind. reflexivity.
 Qed.
 
+(** Add the standard notations for [bind] and [sequence]. *)
+
 Notation "m >>= f" :=
   (bind m f) (left associativity, at level 49).
 
@@ -100,7 +124,7 @@ Proof.
   unfold bind. reflexivity.
 Qed.
 
-(* Not at all this notation is useful given that it appears to sequence only
+(** Not at all this notation is useful given that it appears to sequence only
    two operations and does not support sequence. *)
 
 Notation "'do' a <- e ; c" :=
@@ -113,11 +137,16 @@ Qed.
 
 End definition2.
 
-(** Third attempt that parameterizes State over types. *)
+(** Third attempt that parameterizes [State] over types. Instead of using
+ uninterpreted types for [S] and [A] the are now parameters to the [State]
+ type. *)
 
 Module definition3.
 
 Definition State (S A:Type) := S -> A * S.
+
+(** [unit] and [bind] change only in that [A] and [S] are now inferred types
+  rather than explicitly defined. *)
 
 Definition unit{S A:Type}(x:A):(State S A) := (fun (s:S) => (x,s)).
 
@@ -132,6 +161,9 @@ Definition sequence{S A:Type}(m:(State S A))(n:(State S A)):(State S A) :=
      match (m s0) with
            | (a,s1) => n s1
      end).
+
+(** [put] and [get] are defined for all state monads in addition to [unit]
+ and [bind].  Still need to find the laws for these operations. *)
 
 Definition put{S A:Type}(a:A)(s1:S):(State S A) := (fun (s0:S) => (a,s1)).
 
@@ -174,11 +206,14 @@ Qed.
 
 Print bind_put.
 
-(*
-   This should be parameterized over both A and B allowing f:A->State S B,
-   but something is fouling that up.  Will come back to it later.  Right now
-   State and its functions are monoids and not monads.  Specifically, the
-   associative operator is closed.
+(** Prove the three basic monad laws - left unit, right unit and associativity.
+   None of these proofs is particularly challenging.
+
+   Proofs should be parameterized over both [A] and [B] allowing 
+   [f:A->State S B] to change the output type.
+   Something is fouling that up.  Will come back to it later.  Right now
+   [State] and its functions are a monoid and not a monad.  Specifically, the
+   associative operator, [bind] is closed.
 *)
 
 Theorem left_unit :
@@ -195,8 +230,6 @@ Proof.
   reflexivity.
 Qed.
 
-(* Again should be parameterized over B and C to allow types to change *)
-
 Theorem assoc :
   forall {S A} (ma:(State S A)) (f:A -> (State S A)) (g:A -> (State S A)),
     bind (bind ma f) g = bind ma (fun a => bind (f a) g).
@@ -212,8 +245,14 @@ End definition3.
 
 Module definition4.
 
-(** Making the StateMonad a Monad using the Monad typeclass. *)
+(** Define the [StateMonad] as a typeclass rather than a single type.  This
+ will enable defining things to be state monads rather than defining a single
+ monad.*)
 
+(** Start with typeclass for [Monad] parameterized over the type
+ [M:Type -> Type].  Note that [M] is a single parameter function.
+ Definition is taken original from the web at *find the link* *)
+ 
 Class Monad (M: Type -> Type):Type := 
 {
   unit: forall {A}, A -> M A
@@ -225,7 +264,17 @@ Class Monad (M: Type -> Type):Type :=
               bind (bind ma f) g = bind ma (fun a => bind (f a) g)
 }.
 
+Notation "m >>= f" :=
+  (bind m f) (left associativity, at level 49).
+
+Notation "m >> f" :=
+  (sequence m f) (left associativity, at level 49).
+
 Definition State (S A:Type) := S -> A * S.
+
+(** Define a [StateMonad] as an instance of [Monad]. Note that this includes
+ only the definitions of [unit] and [bind].  [put] and [get] are defined later
+ outside the typeclass.  This is not optimal, but we'll fix it later *)
 
 Instance StateMonad (S:Type) : Monad (State S) :=
 {
@@ -244,12 +293,6 @@ Proof.
   intros. extensionality x. destruct (ma x) as (a,s1). reflexivity.
   intros. extensionality x. destruct (ma x) as (a,s1). reflexivity.
 Defined.
-
-Notation "m >>= f" :=
-  (bind m f) (left associativity, at level 49).
-
-Notation "m >> f" :=
-  (sequence m f) (left associativity, at level 49).
 
 Example unit_ex1 : ((unit 0) 1) = (0,1).
 Proof.
@@ -310,28 +353,54 @@ Qed.
 
 End definition4.
 
-Module definition5.
+Module abelianmonoid.
 
-(** Example from web discussion *)
+(** Example using subclasses from web discussion.  Start with a Semigroup
+and buid up an Abelian Monoid *)
+
+(** A semigroup is a set ([A]) with an associative operator ([op]) *)
 
 Class Semigroup {A : Type} (op : A -> A -> A) : Type := {
   op_associative : forall x y z : A, op x (op y z) = op (op x y) z
 }.
 
-Print Semigroup.
-
+(** Monoid is a semigroup with left and right IDs *)
 Class Monoid `(M : Semigroup) (id : A) : Type := {
   id_ident_left  : forall x : A, op id x = x;
   id_ident_right : forall x : A, op x id = x
 }.
 
-Print Monoid.
-
+(** Abelian monoid is a monoid whose operator is commutative *)
 Class AbelianMonoid `(M : Monoid) : Type := {
   op_commutative : forall x y : A, op x y = op y x
 }.
 
-Print AbelianMonoid.
+Instance ExSemigroup : (Semigroup mult) := {
+}.
+Proof.
+  intros. apply mult_assoc.
+Qed.
+
+Instance ExMonoid : (Monoid ExSemigroup 1) := {
+}.
+Proof.
+  intros. apply mult_1_l.
+  intros. apply mult_1_r.
+Qed.
+
+Instance ExAbMonoid : (AbelianMonoid ExMonoid) :=
+{
+}.
+Proof.
+  intros. apply mult_comm.
+Qed.
+
+End abelianmonoid.
+
+Module definition5.
+
+(** Try the same approach extending the [Monad] typeclass to implement a
+  [StateMonad] typeclass.  [M] is the monad constructor. *)
 
 Class Monad (M: Type -> Type):Type := 
 {
@@ -348,13 +417,13 @@ Definition State (S A:Type) := S -> A * S.
 
 Class StateMonad {S A:Type} (State: Type -> Type -> Type) `(Monad (State S)) :Type :=
 {
-  get: State S A
-  ; put (a:A) (s:S) : State S A
+  get: A -> State S S
+  ; put: S -> A -> State S A
 }.
 
 Print StateMonad.
 
-Instance StateMonadI (S:Type) : Monad (State S) :=
+Instance StateMonadI {S:Type} : Monad (State S) :=
 {
   unit A x := (fun s => (x,s))
   ; bind A B m f := (fun s0 =>
@@ -374,10 +443,10 @@ Defined.
 
 Print StateMonadI.
 
-Instance StateMonadEx (S A:Type) : StateMonad State (StateMonadI S):=
+Instance StateMonadEx {S A:Type} (a:A) : StateMonad State StateMonadI :=
 {
-  put a s := (fun (_:S) => (a,s))
-  ; get := (fun (s:S) => (s,s))
+  put := (fun (s:S) => (fun (a:A) => (fun (_:S) => (a,s))))
+  ; get := (fun (a:A) => (fun (s:S) => (s,s)))
 }.
 
 Print StateMonadEx.
@@ -433,21 +502,38 @@ Qed.
 
 (* Definition put{S A:Type}(s:S)(a:A):(State S A) := (fun (_:S) => (a,s)). *)
 
-Print put
+Eval compute in (put 0 10).
 
-Print unit.
+Eval compute in (fun (a:nat) => (fun (s:nat) => (0,10)):(State nat nat)).
 
-Example put_ex1 : ((unit 1) >>= (put 10)) 0 = (1,10).
+Eval compute in (((unit 1):(State nat nat)) >>= ((fun (a:nat) => (put 0 10):(State nat nat)))) 10.
+
+Example put_ex2: (((unit 1):(State nat nat)) >>= ((fun (a:nat) => (fun (s:nat) => (0,10)):(State nat nat)))) 10 = (0,10).
+Proof.
+  unfold unit, bind.
+  trivial.
+Qed.
+
+Eval compute in ((((unit 1) >>= (put 10)):(State nat nat)) 8).
+
+(* Example put_ex1 : ((((unit 1) >>= (put 10)):(State nat nat)) 8) = (1,10).
 Proof.
   unfold bind. simpl. unfold put. reflexivity.
 Qed.
+*)
 
 (* Definition get{S:Type}(a:S):(State S S) := (fun (s:S) => (s,s)). *)
+
+
+Eval compute in ((unit 0) >>= get).
+
+Check ((unit 0) >>= get).
+
+Eval compute in ((unit 0) >>= get) 10.
 
 Example get_ex1 : ((unit 0) >>= get) 10 = (10,10).
 Proof.
   unfold bind. simpl. unfold get. reflexivity.
 Qed.
-
 
 End definition5.
